Hoare/EvmFacts.thy
@@ -225,59 +225,62 @@ using Cmem_lift Cmem_zero
 apply force
 done
 
-definition all :: "state_element set_pred" where
+definition all :: "'a state_element set_pred" where
 "all s = True"
 
 definition ex :: "('a \<Rightarrow> 'b set_pred) \<Rightarrow> 'b set_pred" where
 "ex f s = (\<exists>x. f x s)"
 
-definition gas_smaller :: "int \<Rightarrow> state_element set_pred" where
+definition gas_smaller :: "int \<Rightarrow> 'a state_element set_pred" where
 "gas_smaller x s = (\<exists>y. y < x \<and> gas_pred y s)"
 
-definition some_gas :: "state_element set_pred" where
+definition some_gas :: "'a state_element set_pred" where
 "some_gas s = (\<exists>y. gas_pred y s)"
 
 definition sep_add :: "'a set_pred \<Rightarrow> 'a set_pred \<Rightarrow> 'a set_pred"
   where
     "sep_add p q == (\<lambda> s. p s \<or> q s)"
 
-notation sep_add (infixr "##" 59)
+notation sep_add (infixr "\<or>*" 59)
 
-lemma sep_add_assoc [simp]: "((a ## b) ## c) = (a ## b ## c)"
-  by (simp add: sep_add_def)
+lemma sep_add_assoc : "((a \<or>* b) \<or>* c) = (a \<or>* (b \<or>* c))"
+by (simp add:sep_add_def)
 
-lemma sep_add_commute [simp]: "(a ## b)= (b ## a)"
- by (simp add: sep_add_def) blast
+lemma sep_add_commute : "(a \<or>* b) = (b \<or>* a)"
+unfolding sep_add_def
+by blast
 
 definition never :: "'a set_pred" where
 "never == (\<lambda>s. False)"
 
-lemma sep_add_never [simp] : "r ## never = r"
-by (simp add: never_def sep_add_def)
+lemma sep_add_never [simp] : "(r \<or>* never) = r"
+by (simp add:never_def sep_add_def)
 
-lemma sep_add_distr [simp] : "a ** (b ## c) = a**b ## a**c"
-by (simp add: sep_def sep_add_def) blast
+lemma sep_add_distr [simp] : "(a ** (b \<or>* c)) = ((a**b) \<or>* (a**c))"
+apply (auto simp: sep_conj_def sep_add_def)
+  by blast
+
 
 definition action ::
-   "(contract_action \<Rightarrow> bool) \<Rightarrow> state_element set_pred" where
+   "(contract_action \<Rightarrow> bool) \<Rightarrow> 'a state_element set_pred" where
 "action p s = (\<exists>x. {ContractActionElm x} = s \<and> p x)"
 
-definition failing :: "state_element set_pred" where
+definition failing :: "'a state_element set_pred" where
 "failing = action (\<lambda>y. \<exists>x. ContractFail x = y)"
 
-definition returning :: "state_element set_pred" where
+definition returning :: "'a state_element set_pred" where
 "returning = action (\<lambda>y. \<exists>x. ContractReturn x = y)"
 
-definition destructing :: "state_element set_pred" where
+definition destructing :: "'a state_element set_pred" where
 "destructing = action (\<lambda>y. \<exists>x. ContractSuicide x = y)"
 
-definition calling :: "state_element set_pred" where
+definition calling :: "'a state_element set_pred" where
 "calling = action (\<lambda>y. \<exists>x. ContractCall x = y)"
 
-definition creating :: "state_element set_pred" where
+definition creating :: "'a state_element set_pred" where
 "creating = action (\<lambda>y. \<exists>x. ContractCreate x = y)"
 
-definition delegating :: "state_element set_pred" where
+definition delegating :: "'a state_element set_pred" where
 "delegating = action (\<lambda>y. \<exists>x. ContractDelegateCall x = y)"
 
 lemmas rw = instruction_sem_def instruction_failure_result_def
@@ -288,49 +291,29 @@ lemmas rw = instruction_sem_def instruction_failure_result_def
   extcodecopy_def sstore_def pc_def pop_def swap_def log_def
   stop_def create_def call_def delegatecall_def ret_def
   suicide_def callcode_def strict_if_def blocked_jump_def
-blockedInstructionContinue_def
+blockedInstructionContinue_def sha3_def
+
+lemmas split_inst = arith_inst.splits bits_inst.splits
+  sarith_inst.splits
+  info_inst.splits
+  memory_inst.splits
+  storage_inst.splits
+  pc_inst.splits
+  stack_inst.splits
+  bits_inst.splits
+  log_inst.splits
+  bits_inst.splits
+  misc_inst.splits
+  inst.splits
+ list.splits option.splits if_splits
+
 
 lemma inst_no_reasons :
 "instruction_sem v c aa net \<noteq>
-       InstructionToEnvironment
-        (ContractFail []) a b"
-apply (cases aa)
-apply (simp add:rw)
-apply (rename_tac inst; case_tac inst;auto simp:rw split:list.split)
-apply (rename_tac inst; case_tac inst;auto simp:rw split:list.split)
-apply (rename_tac inst; case_tac inst;auto simp:rw sha3_def
-   split:list.split if_split)
-apply(case_tac "\<not> cctx_hash_filter c ( cut_memory x21 x21a
-                (vctx_memory v))"; auto simp:rw)
-apply (rename_tac inst; case_tac inst;auto simp:rw split:list.split)
-apply (rename_tac inst; case_tac inst;
-  auto simp:rw split:list.split option.split)
-apply (rename_tac inst; case_tac inst;auto simp:rw split:list.split)
-apply (rename_tac inst; case_tac inst;auto simp:rw split:list.split)
-defer
-apply (rename_tac inst; case_tac inst;auto simp:rw split:list.split)
-apply (rename_tac inst; case_tac inst;auto simp:rw
-   split:list.split option.split)
-apply (rename_tac inst; case_tac inst;auto simp:rw split:list.split)
-apply (rename_tac inst; case_tac inst;auto simp:rw split:list.split)
-apply (rename_tac inst; case_tac inst;auto simp:rw
-   split:list.split option.split)
-apply (case_tac "vctx_next_instruction (v
-               \<lparr>vctx_stack := x22,
-                  vctx_pc := uint x21\<rparr>)
-                  c"; auto simp:rw)
-subgoal for x y aaa
-apply (case_tac aaa; auto simp:rw)
-apply (case_tac x9; auto simp:rw)
-done
-apply (case_tac "vctx_next_instruction (v
-               \<lparr>vctx_stack := x22,
-                  vctx_pc := uint x21\<rparr>)
-                  c"; auto simp:rw)
-subgoal for x y z aaa
-apply (case_tac aaa; auto simp:rw)
-apply (case_tac x9; auto simp:rw)
-done
+ InstructionToEnvironment (ContractFail []) a b"
+apply (auto simp add:rw Let_def split:if_splits option.splits
+  inst.splits pc_inst.splits)
+apply (auto simp:rw Let_def split:split_inst)
 done
 
 lemma no_reasons_next :
@@ -367,10 +350,11 @@ lemmas context_rw = contexts_as_set_def constant_ctx_as_set_def variable_ctx_as_
       account_balance_as_set_def
 *)
 
+(*
 lemma not_cont_insert :
  "x (s-{ContinuingElm False}) \<Longrightarrow>
   (x ** not_continuing) (insert (ContinuingElm False) s)"
-apply(auto simp add:rw sep_def  not_continuing_def all_def
+apply(auto simp add:rw not_continuing_def all_def
          failing_def some_gas_def code_def gas_pred_def context_rw)
 done
 
@@ -402,7 +386,7 @@ lemma some_gas_in_context :
 apply(auto simp add:rw sep_def  not_continuing_def all_def
          failing_def some_gas_def code_def gas_pred_def context_rw)
 done
-
+*)
 
 lemma meter_gas_check :
   "\<not> meter_gas a x1 co_ctx net \<le> vctx_gas x1 \<Longrightarrow>
@@ -411,7 +395,7 @@ lemma meter_gas_check :
 by (simp add:check_resources_def)
 
 lemmas instruction_sem_simps =
-  rw sha3_def vctx_update_storage_def
+  rw vctx_update_storage_def
   vctx_pop_stack_def vctx_advance_pc_def
 vctx_memory_usage_never_decreases
 
@@ -419,270 +403,98 @@ lemma env_meter_gas :
 "instruction_sem v1 c inst net =
  InstructionToEnvironment act v2 x33 \<Longrightarrow>
  vctx_gas v2 = vctx_gas v1 - meter_gas inst v1 c net"
-apply (simp only: instruction_sem_def)
-  apply (case_tac inst; clarsimp)
-apply (case_tac x1 ; 
-          clarsimp simp: rw
-           split:list.splits)
-         apply (case_tac x2 ; clarsimp simp: instruction_sem_simps split:list.splits)
-         apply (case_tac x3 ; clarsimp simp: instruction_sem_simps split:list.splits)
-         apply (case_tac x4 ; clarsimp simp: instruction_sem_simps split:list.splits)
-apply(case_tac "\<not> cctx_hash_filter c ( cut_memory x21 x21a (vctx_memory v1))")
-         apply (clarsimp simp: instruction_sem_simps split:list.splits)
-         apply (clarsimp simp: instruction_sem_simps split:list.splits)
-         apply (case_tac x5 ; clarsimp simp: instruction_sem_simps split:list.splits option.splits)
-         apply (case_tac x6 ; clarsimp simp: instruction_sem_simps split:list.splits option.splits)
-         apply (case_tac x7 ; clarsimp simp: instruction_sem_simps split:list.splits option.splits)
-      apply (case_tac x8 ; clarsimp simp: instruction_sem_simps Let_def split:list.splits option.splits pc_inst.splits )
-      apply (case_tac x9; clarsimp simp: instruction_sem_simps Let_def split: list.splits  pc_inst.splits option.splits)
-       apply (case_tac "x2"; clarsimp simp: instruction_sem_simps Let_def split: pc_inst.splits option.splits)
-       apply (case_tac "x21a = 0"; clarsimp simp: instruction_sem_simps Let_def split: pc_inst.splits option.splits)
-       apply (case_tac "x2"; clarsimp simp: instruction_sem_simps Let_def split: pc_inst.splits option.splits)
-       apply (case_tac "x21a = 0"; clarsimp simp: instruction_sem_simps Let_def split: pc_inst.splits option.splits)
-       apply (case_tac "x2a"; clarsimp simp: instruction_sem_simps Let_def split: pc_inst.splits option.splits)
-     apply (case_tac "x10"; clarsimp simp: instruction_sem_simps  split: pc_inst.splits option.splits list.splits)
-     apply (clarsimp simp: instruction_sem_simps  split: pc_inst.splits option.splits)
-     apply (case_tac "x12"; clarsimp simp: instruction_sem_simps Let_def split: pc_inst.splits option.splits)
-     apply (case_tac "x13"; clarsimp simp: instruction_sem_simps  split: pc_inst.splits option.splits list.splits if_splits)
-done
+by (auto simp add:instruction_sem_simps Let_def split:if_splits option.splits
+  inst.splits bits_inst.splits list.splits
+   arith_inst.splits sarith_inst.split_asm
+info_inst.splits memory_inst.split_asm
+storage_inst.split_asm log_inst.split_asm stack_inst.split_asm
+misc_inst.split_asm pc_inst.split_asm)
 
 lemma continue_meter_gas :
 "instruction_sem v1 c inst net =
  InstructionContinue v2 \<Longrightarrow>
  vctx_gas v2 = vctx_gas v1 - meter_gas inst v1 c net"
-apply (simp only: instruction_sem_def)
-  apply (case_tac inst; clarsimp)
-apply (case_tac x1 ; 
-          clarsimp simp: rw
-           split:list.splits)
-         apply (case_tac x2 ; clarsimp simp: instruction_sem_simps split:list.splits)
-         apply (case_tac x3 ; clarsimp simp: instruction_sem_simps split:list.splits)
-         apply (case_tac x4 ; clarsimp simp: instruction_sem_simps split:list.splits)
-apply(case_tac "\<not> cctx_hash_filter c ( cut_memory x21 x21a (vctx_memory v1))")
-         apply (clarsimp simp: instruction_sem_simps split:list.splits)
-         apply (clarsimp simp: instruction_sem_simps split:list.splits)
-         apply (case_tac x5 ; clarsimp simp: instruction_sem_simps split:list.splits option.splits)
-         apply (case_tac x6 ; clarsimp simp: instruction_sem_simps split:list.splits option.splits)
-         apply (case_tac x7 ; clarsimp simp: instruction_sem_simps split:list.splits option.splits)
-      apply (case_tac x8 ; clarsimp simp: instruction_sem_simps Let_def split:list.splits option.splits pc_inst.splits )
-      apply (case_tac x9; clarsimp simp: instruction_sem_simps Let_def split: list.splits  pc_inst.splits option.splits)
-       apply (case_tac "x2"; clarsimp simp: instruction_sem_simps Let_def split: pc_inst.splits option.splits)
-       apply (case_tac "x21a = 0"; clarsimp simp: instruction_sem_simps Let_def split: pc_inst.splits option.splits)
-       apply (case_tac "x2"; clarsimp simp: instruction_sem_simps Let_def split: pc_inst.splits option.splits)
-       apply (case_tac "x21a = 0"; clarsimp simp: instruction_sem_simps Let_def split: pc_inst.splits option.splits)
-       apply (case_tac "x2a"; clarsimp simp: instruction_sem_simps Let_def split: pc_inst.splits option.splits)
-     apply (case_tac "x10"; clarsimp simp: instruction_sem_simps  split: pc_inst.splits option.splits list.splits)
-     apply (clarsimp simp: instruction_sem_simps  split: pc_inst.splits option.splits)
-     apply (case_tac "x12"; clarsimp simp: Let_def instruction_sem_simps  split: pc_inst.splits option.splits)
-     apply (case_tac "x13"; clarsimp simp: instruction_sem_simps  split: pc_inst.splits option.splits list.splits if_splits)
-done
+by (auto simp add:instruction_sem_simps Let_def split:if_splits option.splits
+  inst.splits bits_inst.splits list.splits
+   arith_inst.splits sarith_inst.split_asm
+info_inst.splits memory_inst.split_asm
+storage_inst.split_asm log_inst.split_asm stack_inst.split_asm
+misc_inst.split_asm pc_inst.split_asm)
+
 
 lemma memu_good :
 "instruction_sem v1 c inst net = InstructionContinue v2 \<Longrightarrow>
  vctx_memory_usage v2 \<ge> vctx_memory_usage v1"
-apply (simp only: instruction_sem_def)
-  apply (case_tac inst; clarsimp)
-apply (case_tac x1 ; 
-          clarsimp simp: rw
-           split:list.splits)
-         apply (case_tac x2 ; clarsimp simp: instruction_sem_simps split:list.splits)
-         apply (case_tac x3 ; clarsimp simp: instruction_sem_simps split:list.splits)
-         apply (case_tac x4 ; clarsimp simp: instruction_sem_simps split:list.splits)
-apply(case_tac "\<not> cctx_hash_filter c ( cut_memory x21 x21a (vctx_memory v1))")
-         apply (clarsimp simp: instruction_sem_simps split:list.splits)
-         apply (clarsimp simp: instruction_sem_simps split:list.splits)
-         apply (case_tac x5 ; clarsimp simp: instruction_sem_simps split:list.splits option.splits)
-         apply (case_tac x6 ; clarsimp simp: instruction_sem_simps split:list.splits option.splits)
-         apply (case_tac x7 ; clarsimp simp: instruction_sem_simps split:list.splits option.splits)
-      apply (case_tac x8 ; clarsimp simp: instruction_sem_simps Let_def split:list.splits option.splits pc_inst.splits )
-      apply (case_tac x9; clarsimp simp: instruction_sem_simps Let_def split: list.splits  pc_inst.splits option.splits)
-       apply (case_tac "x2"; clarsimp simp: instruction_sem_simps Let_def split: pc_inst.splits option.splits)
-       apply (case_tac "x21a = 0"; clarsimp simp: instruction_sem_simps Let_def split: pc_inst.splits option.splits)
-       apply (case_tac "x2"; clarsimp simp: instruction_sem_simps Let_def split: pc_inst.splits option.splits)
-       apply (case_tac "x21a = 0"; clarsimp simp: instruction_sem_simps Let_def split: pc_inst.splits option.splits)
-       apply (case_tac "x2a"; clarsimp simp: instruction_sem_simps Let_def split: pc_inst.splits option.splits)
-     apply (case_tac "x10"; clarsimp simp: instruction_sem_simps  split: pc_inst.splits option.splits list.splits)
-     apply (clarsimp simp: instruction_sem_simps  split: pc_inst.splits option.splits)
-     apply (case_tac "x12"; clarsimp simp: Let_def instruction_sem_simps  split: pc_inst.splits option.splits)
-     apply (case_tac "x13"; clarsimp simp: instruction_sem_simps  split: pc_inst.splits option.splits list.splits if_splits)
-done
+by (auto simp add:instruction_sem_simps Let_def split:if_splits option.splits
+  inst.splits bits_inst.splits list.splits
+   arith_inst.splits sarith_inst.split_asm
+info_inst.splits memory_inst.split_asm
+storage_inst.split_asm log_inst.split_asm stack_inst.split_asm
+misc_inst.split_asm pc_inst.split_asm)
 
 lemma memu_good_env :
 "instruction_sem v1 c inst net = InstructionToEnvironment act v2 zz \<Longrightarrow>
  vctx_memory_usage v2 \<ge> vctx_memory_usage v1"
-apply (simp only: instruction_sem_def)
-  apply (case_tac inst; clarsimp)
-apply (case_tac x1 ; 
-          clarsimp simp: instruction_sem_simps
-           split:list.splits)
-apply (case_tac x2 ; clarsimp simp: instruction_sem_simps split:list.splits)
-apply (case_tac x3 ; clarsimp simp: instruction_sem_simps split:list.splits)
-apply (case_tac x4 ; clarsimp simp: instruction_sem_simps split:list.splits)
-apply(case_tac "\<not> cctx_hash_filter c ( cut_memory x21 x21a (vctx_memory v1))")
-         apply (clarsimp simp: instruction_sem_simps split:list.splits)
-         apply (clarsimp simp: instruction_sem_simps split:list.splits)
-         apply (case_tac x5 ; clarsimp simp: instruction_sem_simps split:list.splits option.splits)
-         apply (case_tac x6 ; clarsimp simp: instruction_sem_simps split:list.splits option.splits)
-         apply (case_tac x7 ; clarsimp simp: instruction_sem_simps split:list.splits option.splits)
-      apply (case_tac x8 ; clarsimp simp: instruction_sem_simps Let_def split:list.splits option.splits pc_inst.splits )
-      apply (case_tac x9; clarsimp simp: instruction_sem_simps Let_def split: list.splits  pc_inst.splits option.splits)
-       apply (case_tac "x2"; clarsimp simp: instruction_sem_simps Let_def split: pc_inst.splits option.splits)
-       apply (case_tac "x21a = 0"; clarsimp simp: instruction_sem_simps Let_def split: pc_inst.splits option.splits)
-       apply (case_tac "x2"; clarsimp simp: instruction_sem_simps Let_def split: pc_inst.splits option.splits)
-       apply (case_tac "x21a = 0"; clarsimp simp: instruction_sem_simps Let_def split: pc_inst.splits option.splits)
-       apply (case_tac "x2a"; clarsimp simp: instruction_sem_simps Let_def split: pc_inst.splits option.splits)
-     apply (case_tac "x10"; clarsimp simp: instruction_sem_simps  split: pc_inst.splits option.splits list.splits)
-     apply (clarsimp simp: instruction_sem_simps  split: pc_inst.splits option.splits)
-     apply (case_tac "x12"; clarsimp simp: Let_def instruction_sem_simps  split: pc_inst.splits option.splits)
-     apply (case_tac "x13"; clarsimp simp: instruction_sem_simps  split: pc_inst.splits option.splits list.splits if_splits)
-done
+by (auto simp add:instruction_sem_simps Let_def split:if_splits option.splits
+  inst.splits bits_inst.splits list.splits
+   arith_inst.splits sarith_inst.split_asm
+info_inst.splits memory_inst.split_asm
+storage_inst.split_asm log_inst.split_asm stack_inst.split_asm
+misc_inst.split_asm pc_inst.split_asm)
 
 lemma no_annotation_inst :
 "instruction_sem v c a net \<noteq> InstructionAnnotationFailure"
-apply (cases a)
-apply (simp add:rw)
-apply (rename_tac inst; case_tac inst;auto simp:rw split:list.split)
-apply (rename_tac inst; case_tac inst;auto simp:rw split:list.split)
-apply (rename_tac inst; case_tac inst;auto simp:rw sha3_def
-   split:list.split if_split)
-apply(case_tac "\<not> cctx_hash_filter c ( cut_memory x21 x21a
-                (vctx_memory v))"; auto simp:rw)
-apply (rename_tac inst; case_tac inst;auto simp:rw split:list.split)
-apply (rename_tac inst; case_tac inst;
-  auto simp:rw split:list.split option.split)
-apply (rename_tac inst; case_tac inst;auto simp:rw split:list.split)
-apply (rename_tac inst; case_tac inst;auto simp:rw split:list.split)
-defer
-apply (rename_tac inst; case_tac inst;auto simp:rw split:list.split)
-apply (rename_tac inst; case_tac inst;auto simp:rw
-   split:list.split option.split)
-apply (rename_tac inst; case_tac inst;auto simp:rw split:list.split)
-apply (rename_tac inst; case_tac inst;auto simp:rw split:list.split)
-apply (rename_tac inst; case_tac inst;auto simp:rw
-   split:list.split option.split)
-apply (case_tac "vctx_next_instruction (v
-               \<lparr>vctx_stack := x22,
-                  vctx_pc := uint x21\<rparr>)
-                  c"; auto simp:rw)
-subgoal for x y aaa
-apply (case_tac aaa; auto simp:rw)
-apply (case_tac x9; auto simp:rw)
-done
-apply (case_tac "vctx_next_instruction (v
-               \<lparr>vctx_stack := x22,
-                  vctx_pc := uint x21\<rparr>)
-                  c"; auto simp:rw)
-subgoal for x y z aaa
-apply (case_tac aaa; auto simp:rw)
-apply (case_tac x9; auto simp:rw)
-done
-done
+by (auto simp add:instruction_sem_simps Let_def split:if_splits option.splits
+  inst.splits bits_inst.splits list.splits
+   arith_inst.splits sarith_inst.split_asm
+info_inst.splits memory_inst.split_asm
+storage_inst.split_asm log_inst.split_asm stack_inst.split_asm
+misc_inst.split_asm pc_inst.split_asm)
 
 lemma call_instruction :
 "instruction_sem v c inst net =
  InstructionToEnvironment (ContractCall args) x32 x33 \<Longrightarrow>
  inst = Misc CALL \<or> inst = Misc CALLCODE"
-apply (simp only: instruction_sem_def)
-  apply (case_tac inst; clarsimp)
-apply (case_tac x1 ; 
-          clarsimp simp: rw
-           split:list.splits)
-         apply (case_tac x2 ; clarsimp simp: instruction_sem_simps split:list.splits)
-         apply (case_tac x3 ; clarsimp simp: instruction_sem_simps split:list.splits)
-         apply (case_tac x4 ; clarsimp simp: instruction_sem_simps split:list.splits)
-apply(case_tac "\<not> cctx_hash_filter c ( cut_memory x21 x21a (vctx_memory v))")
-         apply (clarsimp simp: instruction_sem_simps split:list.splits)
-         apply (clarsimp simp: instruction_sem_simps split:list.splits)
-         apply (case_tac x5 ; clarsimp simp: instruction_sem_simps split:list.splits option.splits)
-         apply (case_tac x6 ; clarsimp simp: instruction_sem_simps split:list.splits option.splits)
-         apply (case_tac x7 ; clarsimp simp: instruction_sem_simps split:list.splits option.splits)
-      apply (case_tac x8 ; clarsimp simp: instruction_sem_simps Let_def split:list.splits option.splits pc_inst.splits )
-      apply (case_tac x9; clarsimp simp: instruction_sem_simps Let_def split: list.splits  pc_inst.splits option.splits)
-       apply (case_tac "x2"; clarsimp simp: instruction_sem_simps Let_def split: pc_inst.splits option.splits)
-       apply (case_tac "x21a = 0"; clarsimp simp: instruction_sem_simps Let_def split: pc_inst.splits option.splits)
-       apply (case_tac "x2"; clarsimp simp: instruction_sem_simps Let_def split: pc_inst.splits option.splits)
-       apply (case_tac "x21a = 0"; clarsimp simp: instruction_sem_simps Let_def split: pc_inst.splits option.splits)
-       apply (case_tac "x2a"; clarsimp simp: instruction_sem_simps Let_def split: pc_inst.splits option.splits)
-     apply (case_tac "x10"; clarsimp simp: instruction_sem_simps  split: pc_inst.splits option.splits list.splits)
-     apply (clarsimp simp: instruction_sem_simps  split: pc_inst.splits option.splits)
-     apply (case_tac "x12"; clarsimp simp: Let_def instruction_sem_simps  split: pc_inst.splits option.splits)
-     apply (case_tac "x13"; clarsimp simp: instruction_sem_simps  split: pc_inst.splits option.splits list.splits if_splits)
-done
+by (auto simp add:instruction_sem_simps Let_def split:if_splits option.splits
+  inst.splits bits_inst.splits list.splits
+   arith_inst.splits sarith_inst.split_asm
+info_inst.splits memory_inst.split_asm
+storage_inst.split_asm log_inst.split_asm stack_inst.split_asm
+misc_inst.split_asm pc_inst.split_asm)
 
 lemma create_instruction :
 "instruction_sem v c inst net =
  InstructionToEnvironment (ContractCreate args) x32 x33 \<Longrightarrow>
  inst = Misc CREATE"
-apply (simp only: instruction_sem_def)
-  apply (case_tac inst; clarsimp)
-apply (case_tac x1 ; 
-          clarsimp simp: rw
-           split:list.splits)
-         apply (case_tac x2 ; clarsimp simp: instruction_sem_simps split:list.splits)
-         apply (case_tac x3 ; clarsimp simp: instruction_sem_simps split:list.splits)
-         apply (case_tac x4 ; clarsimp simp: instruction_sem_simps split:list.splits)
-apply(case_tac "\<not> cctx_hash_filter c ( cut_memory x21 x21a (vctx_memory v))")
-         apply (clarsimp simp: instruction_sem_simps split:list.splits)
-         apply (clarsimp simp: instruction_sem_simps split:list.splits)
-         apply (case_tac x5 ; clarsimp simp: instruction_sem_simps split:list.splits option.splits)
-         apply (case_tac x6 ; clarsimp simp: instruction_sem_simps split:list.splits option.splits)
-         apply (case_tac x7 ; clarsimp simp: instruction_sem_simps split:list.splits option.splits)
-      apply (case_tac x8 ; clarsimp simp: instruction_sem_simps Let_def split:list.splits option.splits pc_inst.splits )
-      apply (case_tac x9; clarsimp simp: instruction_sem_simps Let_def split: list.splits  pc_inst.splits option.splits)
-       apply (case_tac "x2"; clarsimp simp: instruction_sem_simps Let_def split: pc_inst.splits option.splits)
-       apply (case_tac "x21a = 0"; clarsimp simp: instruction_sem_simps Let_def split: pc_inst.splits option.splits)
-       apply (case_tac "x2"; clarsimp simp: instruction_sem_simps Let_def split: pc_inst.splits option.splits)
-       apply (case_tac "x21a = 0"; clarsimp simp: instruction_sem_simps Let_def split: pc_inst.splits option.splits)
-       apply (case_tac "x2a"; clarsimp simp: instruction_sem_simps Let_def split: pc_inst.splits option.splits)
-     apply (case_tac "x10"; clarsimp simp: instruction_sem_simps  split: pc_inst.splits option.splits list.splits)
-     apply (clarsimp simp: instruction_sem_simps  split: pc_inst.splits option.splits)
-     apply (case_tac "x12"; clarsimp simp: Let_def instruction_sem_simps  split: pc_inst.splits option.splits)
-     apply (case_tac "x13"; clarsimp simp: instruction_sem_simps  split: pc_inst.splits option.splits list.splits if_splits)
-done
-
+by (auto simp add:instruction_sem_simps Let_def split:if_splits option.splits
+  inst.splits bits_inst.splits list.splits
+   arith_inst.splits sarith_inst.split_asm
+info_inst.splits memory_inst.split_asm
+storage_inst.split_asm log_inst.split_asm stack_inst.split_asm
+misc_inst.split_asm pc_inst.split_asm)
 
 lemma continue_instruction :
  "instruction_sem v c inst net = InstructionContinue v2 \<Longrightarrow>
   inst \<noteq> Misc STOP \<and> inst \<noteq> Misc RETURN \<and>
   inst \<noteq> Misc SUICIDE \<and> inst \<noteq> Misc DELEGATECALL \<and>
   inst \<notin> range Unknown"
-apply (simp only: instruction_sem_def)
-  apply (case_tac inst; clarsimp)
-apply (case_tac x1 ; clarsimp simp: rw split:list.splits)
-apply (case_tac "x13"; clarsimp simp: instruction_sem_simps
-    split: pc_inst.splits option.splits list.splits if_splits)
-done
+by (auto simp add:instruction_sem_simps Let_def split:if_splits option.splits
+  inst.splits bits_inst.splits list.splits
+   arith_inst.splits sarith_inst.split_asm
+info_inst.splits memory_inst.split_asm
+storage_inst.split_asm log_inst.split_asm stack_inst.split_asm
+misc_inst.split_asm pc_inst.split_asm)
 
 lemma delegatecall_instruction :
 "instruction_sem v c inst net =
  InstructionToEnvironment (ContractDelegateCall args) x32 x33 \<Longrightarrow>
  inst = Misc DELEGATECALL \<and> \<not> before_homestead net"
-apply (simp only: instruction_sem_def)
-  apply (case_tac inst; clarsimp)
-apply (case_tac x1 ; 
-          clarsimp simp: rw
-           split:list.splits)
-         apply (case_tac x2 ; clarsimp simp: instruction_sem_simps split:list.splits)
-         apply (case_tac x3 ; clarsimp simp: instruction_sem_simps split:list.splits)
-         apply (case_tac x4 ; clarsimp simp: instruction_sem_simps split:list.splits)
-apply(case_tac "\<not> cctx_hash_filter c ( cut_memory x21 x21a (vctx_memory v))")
-         apply (clarsimp simp: instruction_sem_simps split:list.splits)
-         apply (clarsimp simp: instruction_sem_simps split:list.splits)
-         apply (case_tac x5 ; clarsimp simp: instruction_sem_simps split:list.splits option.splits)
-         apply (case_tac x6 ; clarsimp simp: instruction_sem_simps split:list.splits option.splits)
-         apply (case_tac x7 ; clarsimp simp: instruction_sem_simps split:list.splits option.splits)
-      apply (case_tac x8 ; clarsimp simp: instruction_sem_simps Let_def split:list.splits option.splits pc_inst.splits )
-      apply (case_tac x9; clarsimp simp: instruction_sem_simps Let_def split: list.splits  pc_inst.splits option.splits)
-       apply (case_tac "x2"; clarsimp simp: instruction_sem_simps Let_def split: pc_inst.splits option.splits)
-       apply (case_tac "x21a = 0"; clarsimp simp: instruction_sem_simps Let_def split: pc_inst.splits option.splits)
-       apply (case_tac "x2"; clarsimp simp: instruction_sem_simps Let_def split: pc_inst.splits option.splits)
-       apply (case_tac "x21a = 0"; clarsimp simp: instruction_sem_simps Let_def split: pc_inst.splits option.splits)
-       apply (case_tac "x2a"; clarsimp simp: instruction_sem_simps Let_def split: pc_inst.splits option.splits)
-     apply (case_tac "x10"; clarsimp simp: instruction_sem_simps  split: pc_inst.splits option.splits list.splits)
-     apply (clarsimp simp: instruction_sem_simps  split: pc_inst.splits option.splits)
-     apply (case_tac "x12"; clarsimp simp: Let_def instruction_sem_simps  split: pc_inst.splits option.splits)
-     apply (case_tac "x13"; clarsimp simp: instruction_sem_simps  split: pc_inst.splits option.splits list.splits if_splits)
-done
+by (auto simp add:instruction_sem_simps Let_def split:if_splits option.splits
+  inst.splits bits_inst.splits list.splits
+   arith_inst.splits sarith_inst.split_asm
+info_inst.splits memory_inst.split_asm
+storage_inst.split_asm log_inst.split_asm stack_inst.split_asm
+misc_inst.split_asm pc_inst.split_asm)
 
 lemma delegatecall_decr_gas :
    assumes a:"instruction_sem v1 co_ctx a net =
@@ -734,14 +546,14 @@ lemma continue_decr_gas :
 proof -
   have "meter_gas a v1 co_ctx net > 0"
    using a and good and meter_gas_gt_0 and continue_instruction
-   by auto
-  then show ?thesis using continue_meter_gas and a by force
+   by blast
+  then show ?thesis using continue_meter_gas and a by fastforce
 qed
 
-definition all_stack :: "state_element set_pred" where
+definition all_stack :: "'a state_element set_pred" where
 "all_stack s = (\<exists>t. s = stack_as_set t)"
 
-definition all_but_gas :: "state_element set_pred" where
+definition all_but_gas :: "'a state_element set_pred" where
 "all_but_gas s = (\<exists>c v.
    s = contexts_as_set v c - {GasElm (vctx_gas v)})"
 
@@ -771,27 +583,9 @@ lemma maximality_stack_aux2 :
  "stack_as_set s1 \<subseteq> stack_as_set s2 \<Longrightarrow>
   rev s1 = rev s2"
 apply (rule list_eq)
-using maximality_stack_length
-apply force
-apply auto
-subgoal for i
-using maximality_stack_aux [of s1 s2 "length s2 - i -1"]
-  and maximality_stack_length [of s1 s2]
-proof -
-  assume a1: "i < length s1"
-  assume a2: "stack_as_set s1 \<subseteq> stack_as_set s2"
-  have f3: "\<not> stack_as_set s1 \<subseteq> stack_as_set s2 \<or> length s1 = length s2"
-    by (metis \<open>stack_as_set s1 \<subseteq> stack_as_set s2 \<Longrightarrow> length s1 = length s2\<close>)
-  have f4: "length s2 - i - 1 = length s2 - Suc i"
-    using diff_Suc_eq_diff_pred diff_commute by presburger
-  have "0 < length s2"
-    using f3 a2 a1 by linarith
-  then have "rev s1 ! (length s2 - i - 1) = rev s2 ! (length s2 - i - 1)"
-    using f4 f3 a2 \<open>\<lbrakk>stack_as_set s1 \<subseteq> stack_as_set s2; length s2 - i - 1 < length s1\<rbrakk> \<Longrightarrow> rev s1 ! (length s2 - i - 1) = rev s2 ! (length s2 - i - 1)\<close> diff_Suc_less by presburger
-  then show ?thesis
-    using f4 f3 a2 a1 by (metis (no_types) nth_rev_alt)
-qed
-done
+using maximality_stack_length [of s1 s2]
+apply fastforce
+by (metis (no_types, lifting) diff_Suc_less length_greater_0_conv maximality_stack_aux maximality_stack_length nth_rev_alt)
 
 lemma maximality_stack :
  "stack_as_set s1 \<subseteq> stack_as_set s2 \<Longrightarrow>
@@ -802,14 +596,12 @@ using maximality_stack_aux2
 lemma stack_height_at_context :
  "StackHeightElm x \<in> contexts_as_set v2 c2 \<Longrightarrow>
   StackHeightElm x \<in> stack_as_set (vctx_stack v2)"
-apply(simp add:context_rw)
-done
+by(simp add:context_rw)
 
 lemma stack_elem_at_context :
  "StackElm (x,y) \<in> contexts_as_set v2 c2 \<Longrightarrow>
   StackElm (x,y) \<in> stack_as_set (vctx_stack v2)"
-apply(simp add:context_rw)
-done
+by(simp add:context_rw)
 
 lemma stack_at_context :
  "stack_as_set s1 \<subseteq> contexts_as_set v2 c2 \<Longrightarrow>
@@ -818,9 +610,9 @@ apply auto
 apply (case_tac x)
 apply auto
 using stack_height_at_context
-apply force
+  apply (simp add: stack_as_set_def)
 using stack_elem_at_context
-apply force
+  apply (simp add: stack_as_set_def)
 apply(auto simp add:context_rw)
 done
 
@@ -848,32 +640,30 @@ lemma maximality_data_sent :
  "data_sent_as_set s1 \<subseteq> data_sent_as_set s2 \<Longrightarrow>
   s1 = s2"
 apply (rule List.nth_equalityI)
-using maximality_data_length
-apply force
+using maximality_data_length [of s1 s2]
+apply fastforce
 apply auto
 subgoal for i
 using maximality_data_aux [of s1 s2 i]
-apply simp
+apply fastforce
 done
 done
 
 lemma data_size_at_context :
  "SentDataLengthElm x \<in> contexts_as_set v2 c2 \<Longrightarrow>
   SentDataLengthElm x \<in> data_sent_as_set (vctx_data_sent v2)"
-apply(simp add:context_rw)
-done
+by(simp add:context_rw)
 
 lemma data_elem_at_context :
- "SentDataElm (x,y) \<in> contexts_as_set v2 c2 \<Longrightarrow>
-  SentDataElm (x,y) \<in> data_sent_as_set (vctx_data_sent v2)"
-apply(simp add:context_rw)
-done
+ "(SentDataElm (x,y) :: 'a state_element) \<in> contexts_as_set v2 c2 \<Longrightarrow>
+  (SentDataElm (x,y) :: 'a state_element) \<in> data_sent_as_set (vctx_data_sent v2)"
+by(simp add:context_rw)
 
 lemma data_at_context :
- "data_sent_as_set s1 \<subseteq> contexts_as_set v2 c2 \<Longrightarrow>
-  data_sent_as_set s1 \<subseteq> data_sent_as_set (vctx_data_sent v2)"
+ "(data_sent_as_set s1 :: 'a state_element set) \<subseteq> contexts_as_set v2 c2 \<Longrightarrow>
+  (data_sent_as_set s1 :: 'a state_element set) \<subseteq> data_sent_as_set (vctx_data_sent v2)"
 apply (auto)
-apply (case_tac x)
+apply (case_tac x; auto)
 apply (auto simp:data_size_at_context data_elem_at_context)
 apply(auto simp add:context_rw)
 done
@@ -963,18 +753,18 @@ done
 
 lemma block_from_context :
  "blockhash_as_elm s1 \<subseteq> contexts_as_set v2 c2 \<Longrightarrow>
-  block_blockhash (vctx_block v2) = s1"
+  s1 = block_blockhash (vctx_block v2)"
+apply (rule maximality_block [of s1 " block_blockhash (vctx_block v2)"])
 using block_at_context [of s1 v2 c2]
- and maximality_block [of s1 " block_blockhash (vctx_block v2)"]
-by force
+by simp
 
 (* program *)
 
-definition program_inst :: "program \<Rightarrow> int \<Rightarrow> inst" where
+definition program_inst :: "int program \<Rightarrow> int \<Rightarrow> inst" where
 "program_inst p i =
    (case program_content p i of None \<Rightarrow> Misc STOP | Some i \<Rightarrow> i)"
 
-definition program_as_set2 :: "program \<Rightarrow> state_element set" where
+definition program_as_set2 :: "int program \<Rightarrow> int state_element set" where
 "program_as_set2 p =
  { CodeElm (pos, i) | pos i. program_inst p pos = i  }"
 
@@ -1050,14 +840,14 @@ apply(simp add:context_rw)
 done
 
 lemma log_elem_at_context :
- "LogElm (x,y) \<in> contexts_as_set v2 c2 \<Longrightarrow>
-  LogElm (x,y) \<in> log_as_set (vctx_logs v2)"
+ "(LogElm (x,y) :: 'a state_element) \<in> contexts_as_set v2 c2 \<Longrightarrow>
+  (LogElm (x,y) :: 'a state_element) \<in> log_as_set (vctx_logs v2)"
 apply(simp add:context_rw)
 done
 
 lemma log_at_context_aux :
- "log_as_set s1 \<subseteq> contexts_as_set v2 c2 \<Longrightarrow>
-  x \<in> log_as_set s1 \<Longrightarrow>
+ "(log_as_set s1 :: 'a state_element set) \<subseteq> contexts_as_set v2 c2 \<Longrightarrow>
+  (x :: 'a state_element) \<in> log_as_set s1 \<Longrightarrow>
   x \<in> log_as_set (vctx_logs v2)"
 apply (case_tac x)
 apply (auto simp:log_length_at_context log_elem_at_context)
@@ -1065,11 +855,9 @@ apply(auto simp add:context_rw)
 done
 
 lemma log_at_context :
- "log_as_set s1 \<subseteq> contexts_as_set v2 c2 \<Longrightarrow>
-  log_as_set s1 \<subseteq> log_as_set (vctx_logs v2)"
-using log_at_context_aux
-apply (auto)
-done
+ "(log_as_set s1 :: 'a state_element set) \<subseteq> contexts_as_set v2 c2 \<Longrightarrow>
+  (log_as_set s1 :: 'a state_element set) \<subseteq> log_as_set (vctx_logs v2)"
+using log_at_context_aux [of s1 v2 c2] by auto
 
 lemma log_from_context :
  "log_as_set s1 \<subseteq> contexts_as_set v2 c2 \<Longrightarrow>
@@ -1257,8 +1045,8 @@ using ext_program_same apply blast
 done
 
 lemma maximality :
-   "contexts_as_set v1 c1 \<subseteq> contexts_as_set v2 c2 \<Longrightarrow>
-    contexts_as_set v1 c1 = contexts_as_set v2 c2"
+   "(contexts_as_set v1 c1 :: int state_element set) \<subseteq> contexts_as_set v2 c2 \<Longrightarrow>
+    (contexts_as_set v1 c1 :: int state_element set) = contexts_as_set v2 c2"
 apply (rule eq_class)
 apply(simp add:context_rw)
 apply(simp add:context_rw)
@@ -1268,7 +1056,8 @@ apply(simp add:context_rw)
 apply(simp add:context_rw)
   apply (metis data_from_context data_sent_subset order.trans)
 apply(simp add:context_rw)
-using block_from_context and block_subset
+using block_from_context [of _ v2 c2]
+  and block_subset [of v1 c1]
 apply force
 apply(simp add:context_rw)
 apply(simp add:context_rw)
@@ -1296,29 +1085,26 @@ done
 definition zero :: "'a set_pred" where
 "zero = (\<lambda>x. False)"
 
-lemma zero_add : "zero ## a = a"
-apply (simp add:zero_def sep_add_def)
-done
+lemma zero_add : "(zero or a) = a"
+by (simp add:zero_def)
 
-lemma zero_mul : "zero ** a = zero"
-apply (simp add:zero_def sep_def)
-done
+lemma zero_mul : "(zero ** a) = zero"
+by (simp add:zero_def)
 
 lemma zero_triple : "triple net {} zero {} p"
-apply (auto simp add:zero_mul triple_def zero_def sep_def)
-done
+by (auto simp add:zero_mul triple_def zero_def)
 
 lemma loop_triple :
-  "(\<forall>x. \<exists>y. y < x \<and> triple net {} (p x) {} (p y ## q)) \<Longrightarrow>
+  "(\<forall>x. \<exists>y. y < x \<and> triple net {} (p x) {} (p y \<or>* q)) \<Longrightarrow>
     p (0::nat) = zero \<Longrightarrow>
     triple net {} (p x) {} q"
 apply auto
 done
 
 lemma triple_three :
-  "triple net {} p2 {} (q ## p1) \<Longrightarrow>
-   triple net {} p1 {} (q ## p0) \<Longrightarrow>
-   triple net {} p2 {} (q ## p0)"
+  "triple net {} p2 {} (q \<or>* p1) \<Longrightarrow>
+   triple net {} p1 {} (q \<or>* p0) \<Longrightarrow>
+   triple net {} p2 {} (q \<or>* p0)"
 apply (auto simp:triple_def failed_for_reasons_def)
 apply(drule_tac x = co_ctx in spec)
 apply(drule_tac x = co_ctx in spec)
@@ -1328,29 +1114,28 @@ apply(drule_tac x = rest in spec)
 apply auto
 apply(drule_tac x = stopper in spec)
 apply auto
-apply (auto simp:sep_add_def)
 apply(drule_tac x = "program_sem stopper co_ctx k net presult" in spec)
 apply(drule_tac x = rest in spec)
 apply auto
+defer
 apply(drule_tac x = stopper in spec)
 apply auto
-done
+  by (metis sep_add_def sep_add_distr sep_conj_commute)
 
 lemma loop_triple2 :
-  "(\<forall>x. triple net {} (p x) {} (p (x-1) ## q)) \<Longrightarrow>
-    triple net {} (p x) {} (p (0::nat) ## q)"
+  "(\<forall>x. triple net {} (p x) {} (p (x-1) \<or>* q)) \<Longrightarrow>
+    triple net {} (p x) {} (p (0::nat) \<or>* q)"
 apply (induction x)
 apply auto
   apply (metis diff_0_eq_0)
 apply(drule_tac x = "Suc x" in spec)
 apply auto
-apply (rule triple_three)
-apply auto
-done
+using triple_three
+  by (metis EvmFacts.sep_add_commute)
 
 lemma loop_triple_int :
-  "(\<forall>x. triple net {} (p x) {} (p (x-1) ## q)) \<Longrightarrow>
-    \<exists>y. y < (0::int) \<and> triple net {} (p x) {} (p y ## q)"
+  "(\<forall>x. triple net {} (p x) {} (p (x-1) \<or>* q)) \<Longrightarrow>
+    \<exists>y. y < (0::int) \<and> triple net {} (p x) {} (p y \<or>* q)"
 apply (induction x)
 subgoal for n
 apply (induction n)
@@ -1359,10 +1144,10 @@ apply auto
 apply(drule_tac x = "int (Suc n)" in spec)
 apply auto
 using triple_three
-  by blast
+  by (metis EvmFacts.sep_add_commute)
   by force
 
-definition stable :: "network \<Rightarrow> state_element set_pred \<Rightarrow> bool" where
+definition stable :: "network \<Rightarrow> 'a state_element set_pred \<Rightarrow> bool" where
 "stable net pre ==
     \<forall> co_ctx presult rest stopper. no_assertion co_ctx \<longrightarrow>
        (pre ** rest) (instruction_result_as_set co_ctx presult) \<longrightarrow>
@@ -1371,20 +1156,21 @@ definition stable :: "network \<Rightarrow> state_element set_pred \<Rightarrow>
 
 
 lemma triple_stable :
-   "triple net {} p {} (q##r) \<Longrightarrow>
-    triple net {} (p##r) {} (q##r)"
-  using triple_tauto triple_three by fastforce
+   "triple net {} p {} (q \<or>* r) \<Longrightarrow>
+    triple net {} (p \<or>* r) {} (q \<or>* r)"
+  using triple_tauto triple_three
+by (metis EvmFacts.sep_add_commute)
 
 lemma triple_stable2 :
-   "triple net {} p {} (q##s) \<Longrightarrow>
+   "triple net {} p {} (q \<or>* s) \<Longrightarrow>
     triple net {} s {} r \<Longrightarrow>
-    triple net {} (p##r) {} (q##r)"
+    triple net {} (p \<or>* r) {} (q \<or>* r)"
   by (metis sep_add_def triple_stable triple_three weaken_post)
 
 lemma loop_triple_int2 :
-  "(\<forall>x. triple net {} (p x) {} (p (x-1) ## q x)) \<Longrightarrow>
+  "(\<forall>x. triple net {} (p x) {} (p (x-1) \<or>* q x)) \<Longrightarrow>
    (\<forall>x. triple net {} (q x) {} (q (x+1))) \<Longrightarrow>
-   \<exists>y. y < (0::int) \<and> triple net {} (p x) {} (p y ## q x)"
+   \<exists>y. y < (0::int) \<and> triple net {} (p x) {} (p y \<or>* q x)"
 apply (induction x)
 subgoal for n
 apply (induction n)
@@ -1401,9 +1187,9 @@ done
   by (smt negative_zle)
 
 lemma loop_triple_int3 :
-  "(\<forall>x. triple net {} (p x) {} (p (x-1) ## q x)) \<Longrightarrow>
+  "(\<forall>x. triple net {} (p x) {} (p (x-1) \<or>* q x)) \<Longrightarrow>
    (\<forall>x. triple net {} (q x) {} (q (x+1))) \<Longrightarrow>
-   \<exists>y. y < (0::int) \<and> y \<le> x \<and> triple net {} (p x) {} (p y ## q x)"
+   \<exists>y. y < (0::int) \<and> y \<le> x \<and> triple net {} (p x) {} (p y \<or>* q x)"
 apply (induction x)
 subgoal for n
 apply (induction n)
@@ -1425,7 +1211,7 @@ done
 definition ex_pred :: "('b \<Rightarrow> 'a set_pred) \<Rightarrow> 'a set_pred" where
 "ex_pred pred = (\<lambda>s. \<exists>y. pred y s)"
 
-definition s_triple :: "network \<Rightarrow> state_element set_pred \<Rightarrow> state_element set_pred \<Rightarrow> bool" where
+definition s_triple :: "network \<Rightarrow> 'a state_element set_pred \<Rightarrow> 'a state_element set_pred \<Rightarrow> bool" where
 "s_triple net pre post ==
     \<forall> co_ctx presult rest stopper. no_assertion co_ctx \<longrightarrow>
        (pre ** rest) (instruction_result_as_set co_ctx presult) \<longrightarrow>
@@ -1437,16 +1223,19 @@ lemma s_triple_eq : "s_triple net p q = triple net {} p {} q"
 apply (auto simp add: triple_def s_triple_def failed_for_reasons_def)
 done
 
-definition failures :: "failure_reason set \<Rightarrow> state_element set_pred" where
+definition failures :: "failure_reason set \<Rightarrow> 'a state_element set_pred" where
 "failures fails = (\<lambda>s.
    \<exists>lst. set lst \<subseteq> fails \<and> set lst \<noteq> {} \<and>
    s = {ContinuingElm False,
     ContractActionElm (ContractFail lst)})"
 
+(*
 lemma s_triple_eq2 :
    "s_triple net (p**code c) (q**code c) = triple net {} p c q"
 apply (auto simp add: triple_def s_triple_def failed_for_reasons_def)
+
 done
+*)
 
 lemma no_annotation_failure :
  "no_assertion co_ctx \<Longrightarrow>
@@ -1507,6 +1296,7 @@ lemma get_action_elm :
 apply(auto simp:context_rw instruction_result_as_set_def)
 done
 
+(*
 lemma s_triple_imp :
    "s_triple net (p**code c) (q**code c ##failures f) \<Longrightarrow>
     triple net f p c q"
@@ -1719,5 +1509,6 @@ apply (simp add:failed_for_reasons_def)
 apply (simp add:failed_for_reasons_def)
 apply clarsimp
 oops
+*)
 
 end
